\input{preamble_ask.tex}
\input{definitions_ask.tex}

\everymath{\displaystyle}

\begin{document}

\section*{Υπόδειξη}

\begin{align*} 
  \int \mathrm{e}^{-x} \sin^{2}{x} \,{dx} &= \int \mathrm{e}^{-x} \frac{1- \cos{2x}
  }{2}  \,{dx} = \frac{1}{2} \int \mathrm{e}^{-x} \,{dx} - \frac{1}{2} \int 
  \mathrm{e}^{-x} \cos{2x} \,{dx} 
\end{align*}
Για το 1ο ολοκλήρωμα έχουμε:
  \[ \int \mathrm{e}^{-x} \,{dx} = - \mathrm{e}^{-x} \]
Για το 2ο ολοκλήρωμα έχουμε:
\begin{align*} 
  \underbrace{\int \mathrm{e}^{-x} \cos{2x} \, dx}_{I} &= \int (- \mathrm{e}^{-x} )' 
  \cos{2x} \,{dx} \\
  &=  - \mathrm{e}^{-x} \cos{2x} - \int - \mathrm{e}^{-x} (\cos{2x} )' \,{dx} \\
  &= - \mathrm{e}^{-x} \cos{2x} + \int \mathrm{e}^{-x} (-2 \sin{2x}) \,{dx}  \\
  &= - \mathrm{e}^{-x} \cos{2x} -2 \int \mathrm{e}^{-x} \sin{2x} \,{dx}  \\
  &= - \mathrm{e}^{-x} \cos{2x} -2 \int (-\mathrm{e}^{-x})' \sin{2x} \,{dx}  \\
  &= - \mathrm{e}^{-x} \cos{2x} -2 \left( - \mathrm{e}^{-x} \sin{2x} - \int - 
  \mathrm{e}^{-x} (\sin{2x} )' \,{dx}\right) \\
  &= - \mathrm{e}^{-x} \cos{2x} -2 \left( - \mathrm{e}^{-x} \sin{2x} + \int  
  \mathrm{e}^{-x} (2\cos{2x} )' \,{dx}\right) \\
  &= - \mathrm{e}^{-x} \cos{2x} -2 \left( - \mathrm{e}^{-x} \sin{2x} + 2 \int  
  \mathrm{e}^{-x} \cos{2x} \,{dx}\right) \\
  &= - \mathrm{e}^{-x} \cos{2x} + 2 \mathrm{e}^{-x} \sin{2x} -4 
  \underbrace{ \int \mathrm{e}^{-x} \cos{2x} \,{dx}}_{I} \Rightarrow \\
  I + 4I &= - \mathrm{e}^{-x} \cos{2x} + 2 \mathrm{e}^{-x} \sin{2x} \Rightarrow \\
  5I &= - \mathrm{e}^{-x} \cos{2x} + 2 \mathrm{e}^{-x} \sin{2x} \Rightarrow \\
  I &= \frac{- \mathrm{e}^{-x} \cos{2x} + 2 \mathrm{e}^{-x} \sin{2x}}{5} 
\end{align*}

Άρα με αντικατάσταση, έχουμε:
\begin{align*}
  \int \mathrm{e}^{-x} \sin^{2}{x} \,{dx} 
  &= -\frac{1}{2} \mathrm{e}^{-x} - \frac{1}{2} 
  \left(\frac{- \mathrm{e}^{-x} \cos{2x} + 2 \mathrm{e}^{-x} \sin{2x}}{5}\right) \\
  &= -\frac{1}{2} \mathrm{e}^{-x} - \frac{1}{2} \mathrm{e}^{-x} 
  \left(\frac{- \cos{2x} + 2 \sin{2x}}{5}\right) \\
  &= \frac{\mathrm{e}^{-x}}{2} \left( \frac{\cos{2x} - 2 \sin{2x}}{5} - 1\right)
\end{align*}

\end{document}
